format-version: 1.2
data-version: go/releases/2019-09-19/imports/ddanat_import.owl
ontology: go/imports/ddanat_import

[Term]
id: DDANAT:0000003
name: aggregation territory
def: "Area covered by a group of chemotactic cells converging toward the same aggregation center. Can reach a diameter of up to 1 cm." []
is_a: DDANAT:0010082 ! whole organism

[Term]
id: DDANAT:0000004
name: loose aggregate
def: "First adherent mass of cells observed during development, relatively flat with indistinct borders." []
synonym: "loose mound" EXACT []
is_a: DDANAT:0010082 ! whole organism
relationship: develops_from DDANAT:0000003 ! aggregation territory

[Term]
id: DDANAT:0000005
name: mound
def: "Hemispherical structure composed of post-aggregative cells that are undergoing differentiation." []
synonym: "pseudoplasmodium" BROAD []
synonym: "tight aggregate" EXACT []
synonym: "tight mound" EXACT []
is_a: DDANAT:0010082 ! whole organism
relationship: develops_from DDANAT:0000004 ! loose aggregate

[Term]
id: DDANAT:0000006
name: tipped mound
def: "Hemispherical structure composed of post-aggregative cells that are undergoing differentiation and that have formed a tip." []
synonym: "pseudoplasmodium" BROAD []
synonym: "tipped aggregate" EXACT []
is_a: DDANAT:0010082 ! whole organism
relationship: develops_from DDANAT:0000005 ! mound

[Term]
id: DDANAT:0000007
name: standing slug
def: "Cylindrical structure that is formed by elongation of the mound under the control of the tip. The elongating tip is called the first finger." []
synonym: "finger" EXACT []
synonym: "first finger" NARROW []
synonym: "pseudoplasmodium" BROAD []
is_a: DDANAT:0010082 ! whole organism
relationship: develops_from DDANAT:0000006 ! tipped mound

[Term]
id: DDANAT:0000009
name: early culminant
def: "Structure formed after the arrest of slug migration formed when cells of the posterior region of the slug move under the tip. Stalk tube formation is initiated at this stage." []
synonym: "culminant" BROAD []
synonym: "mexican hat" NARROW []
synonym: "pseudoplasmodium" BROAD []
is_a: DDANAT:0010082 ! whole organism
relationship: develops_from DDANAT:0000007 ! standing slug

[Term]
id: DDANAT:0000010
name: mid culminant
def: "Structure in which stalk tube formation has progressed down the prespore zone. Basal disc formation begins at this stage, with the migration of pstA and pstB cells to the lower part of the culminant to form the basal disc." []
synonym: "culminant" BROAD []
synonym: "pseudoplasmodium" BROAD []
is_a: DDANAT:0010082 ! whole organism
relationship: develops_from DDANAT:0000009 ! early culminant

[Term]
id: DDANAT:0000011
name: late culminant
def: "Structure in which stalk tube formation has progressed down to the basal disc. The sorogen ascents up the stalk to it apical position during this stage. Terminal differentiation occurs at this stage: death of the stalk cells and encapsulation of the spores." []
synonym: "culminant" BROAD []
synonym: "pseudoplasmodium" RELATED []
is_a: DDANAT:0010082 ! whole organism
relationship: develops_from DDANAT:0000010 ! mid culminant

[Term]
id: DDANAT:0000012
name: fruiting body
def: "Dicty asexual organism which is terminally differentiated and consists of a long stalk on top of which sits the sorus that contains spores. The mature fruiting body measures between 1.5 to 3 mm in height." []
synonym: "sorocarp" EXACT []
is_a: DDANAT:0010082 ! whole organism
relationship: develops_from DDANAT:0000011 ! late culminant

[Term]
id: DDANAT:0000094
name: sorus
def: "Ovoid structure supported by the stalk and that contains the spores." []
synonym: "spore head" EXACT []
is_a: DDANAT:0010085 ! subdivision

[Term]
id: DDANAT:0010001
name: Dictyostelium discoideum anatomical structure
def: "Material anatomical entity that has inherent 3D shape and is generated by coordinated expression of the Dictyostelium discoideum genome." []

[Term]
id: DDANAT:0010082
name: whole organism
def: "Anatomical structure that is an individual member of the Dictyostelium discoideum species and consists of more than one cell." []
is_a: DDANAT:0010001 ! Dictyostelium discoideum anatomical structure

[Term]
id: DDANAT:0010085
name: subdivision
def: "Anatomical structure which is a primary subdivision of whole Dictyostelium organism. The mereological sum of these is the whole organism." []
is_a: DDANAT:0010001 ! Dictyostelium discoideum anatomical structure

[Typedef]
id: develops_from
name: develops_from
xref: develops_from

