format-version: 1.2
data-version: go/releases/2018-11-06/imports/fao_import.owl
ontology: go/imports/fao_import

[Term]
id: FAO:0000001
name: fungal structure
synonym: "fungal structure ontology" RELATED []

[Term]
id: FAO:0000003
name: basidium
def: "A structure directly from which spores are formed following sexual reproduction in a Basidiomycete." []
is_a: FAO:0000052 ! sporangium
relationship: part_of FAO:0000012 ! basidiocarp

[Term]
id: FAO:0000007
name: fruitbody
def: "Any specialized structure which bears or contains sexually or asexually derived spores." []
synonym: "fruiting body" RELATED []
is_a: FAO:0000001 ! fungal structure

[Term]
id: FAO:0000008
name: ascocarp
def: "A structure within which or at the surface of, an ascus develops in Ascomycetes." []
is_a: FAO:0000007 ! fruitbody

[Term]
id: FAO:0000010
name: sporophore
def: "A structure directly within which spores are contained or from which spores are formed." []
synonym: "spore-bearing organ" RELATED []
is_a: FAO:0000001 ! fungal structure

[Term]
id: FAO:0000012
name: basidiocarp
def: "A large fruiting body that is composed of masses of intertwined hyphal elements and produces basidia and basidiospores. The basidiocarp is characteristic of the majority of fungi of the subphylum Basidiomycotina, in which it is the site of karyogamy and meiosis. Mushrooms and toadstools are common examples." []
synonym: "mushroom" RELATED []
is_a: FAO:0000007 ! fruitbody

[Term]
id: FAO:0000014
name: ascus
def: "A sac-like structure containing sexual spores formed by Ascomycotina; mature asci may have little or no cytoplasm or cytoplasmic contents, and no nucleus outside of the spores." []
is_a: FAO:0000052 ! sporangium

[Term]
id: FAO:0000017
name: sexual spore
def: "A spore formed following meiosis. Sometimes following meiosis, prospores may undergo one or more rounds of mitosis before they are fully mature." []
synonym: "meiotically-derived spore" RELATED []
is_a: FAO:0000019 ! spore

[Term]
id: FAO:0000018
name: unicellular structure
def: "An individual cell composed of a plasma membrane, contents internal to the plasma membrane, and any external protective or encapsulating structure." []
synonym: "cell" EXACT []
is_a: FAO:0000001 ! fungal structure

[Term]
id: FAO:0000019
name: spore
def: "A differentiated form of an organism produced during or as a result of an asexual or sexual reproductive process; usually a cell with a thick cell wall that stores and protects one or more nuclei. Spores may be produced in response to, and are characteristically resistant to, adverse environmental conditions." []
is_a: FAO:0000018 ! unicellular structure

[Term]
id: FAO:0000021
name: basidiospore
def: "A thick walled spore that stores and protects one or more nuclei following sexual reproduction in an Basidiomycete; formed externally on extrusions of the basidium." []
is_a: FAO:0000017 ! sexual spore
relationship: part_of FAO:0000003 ! basidium

[Term]
id: FAO:0000022
name: teliospore
def: "A spore with a very thick cell wall and extracellular peptidoglycan spikes that stores and protects one or more nuclei during dormancy in a Basidiomycete." []
is_a: FAO:0000021 ! basidiospore

[Term]
id: FAO:0000023
name: asexual spore
def: "A spore formed following mitosis or mitoses." []
synonym: "mitotically-derived spore" RELATED []
is_a: FAO:0000019 ! spore

[Term]
id: FAO:0000024
name: conidium
def: "An asexual, nonmotile spore formed by higher fungi; conidia are usually made from the side or tip of specialized sporogenous cells and do not form by progressive cleavage of the cytoplasm." []
is_a: FAO:0000023 ! asexual spore

[Term]
id: FAO:0000026
name: uredospore
def: "A thick walled spore that stores and protects one or more nuclei during dispersal following reproduction in an Basidiomycete." []
synonym: "urediniospore" RELATED []
synonym: "urediospore" RELATED []
is_a: FAO:0000021 ! basidiospore

[Term]
id: FAO:0000038
name: macroconidium
def: "The larger of two types of asexual spores formed by some fungi; usually round or oblong." []
is_a: FAO:0000024 ! conidium

[Term]
id: FAO:0000039
name: oospore
def: "An asexual spore formed by Oomycetes; formed upon fertilization of an oosphere." []
is_a: FAO:0000023 ! asexual spore

[Term]
id: FAO:0000041
name: arthroconidium
def: "Cylindrical spore formed by development and compartmentation of hyphae; the hyphae are often supporting blastoconidiophores." []
synonym: "arthrospore" RELATED []
is_a: FAO:0000038 ! macroconidium

[Term]
id: FAO:0000042
name: blastoconidium
def: "An oblong or round asexual reproductive spore formed specifically by budding." []
synonym: "blastospore" RELATED []
synonym: "reproductive blastospore" RELATED []
is_a: FAO:0000038 ! macroconidium

[Term]
id: FAO:0000043
name: conidiophore
def: "A specialized hypha, often aerial, that gives rise to asexual spores, known as conidia." []
relationship: develops_from FAO:0001001 ! hypha

[Term]
id: FAO:0000044
name: sterigma
def: "A small hyphal branch or structure which supports a sporangium, a conidium, or a basidiospore. In species with biseriate (two layered) sterigmata such as A. nidulans, the first layer comprises primary sterigmata (metulae) and the second layer secondary sterigmata (phialides). Some species, e.g. A. fumigatus, A. oryzae, and others, have only phialides." []
synonym: "sterigmata (plural)" EXACT []
relationship: part_of FAO:0000043 ! conidiophore

[Term]
id: FAO:0000045
name: phialide
def: "A specialized cell that buds from a metula on a developing conidiophore. Multiple phialides may bud from each metula. The phialides in turn divide asymmetrically to give rise to chains of conidia." []
synonym: "secondary sterigma" EXACT []
is_a: FAO:0000044 ! sterigma

[Term]
id: FAO:0000046
name: metula
def: "A specialized cell borne on a conidiophore that gives rise to phialides during the process of conidiation." []
synonym: "metulae (plural)" EXACT []
synonym: "primary sterigma" EXACT []
is_a: FAO:0000044 ! sterigma

[Term]
id: FAO:0000047
name: cleistothecium
def: "A completely closed fruiting body formed by some fungi of the Ascomycota, containing asci." []
is_a: FAO:0000008 ! ascocarp

[Term]
id: FAO:0000048
name: Hulle cell
def: "A specialized multinucleate cell that originates from a nest-like aggregation of hyphae during sexual development. Hulle cells serve as nurse cells to the developing cleistothecium. Note that \"Hulle\" is properly written with an umlaut character on the \"u\"." []
relationship: develops_from FAO:0001001 ! hypha

[Term]
id: FAO:0000050
name: conidiophore stalk
def: "The elongated part of the conidiophore that extends, often aerially, from the growth substrate and supports the structures that bear conidia." []
relationship: part_of FAO:0000043 ! conidiophore

[Term]
id: FAO:0000052
name: sporangium
def: "A structure within which spores develop." []
is_a: FAO:0000010 ! sporophore

[Term]
id: FAO:0001001
name: hypha
def: "A threadlike, tubular filamentous fungal structure." []
is_a: FAO:0000001 ! fungal structure

[Typedef]
id: develops_from
name: develops from
xref: RO:0002202
is_transitive: true

[Typedef]
id: part_of
name: part of
xref: BFO:0000050
is_transitive: true

